theories/νType/Notation.v
@@ -6,6 +6,7 @@ Notation "x .2" := (projT2 x) (at level 1, left associativity, format "x .2").
 Notation "x .+1" := (S x) (at level 1, left associativity, format "x .+1").
 Notation "x .+2" := (S (S x)) (at level 1, left associativity, format "x .+2").
 Notation "x .+3" := (S (S (S x))) (at level 1, left associativity, format "x .+3").
+Notation "x .-1" := (pred x) (at level 1, left associativity, format "x .-1").
 
 (** This is in Program.Basics for some strange reason *)
 Arguments id {A} x.
